sha/hmac_common_lemmas.v
@@ -10,7 +10,8 @@ Require Import pure_lemmas.     (* sha *)
 Require Import sha.spec_sha.
 
 Require Import HMAC_functional_prog.
-
+Require Import HMAC256_functional_prog.
+(*
 Lemma SF_ByteRepr x: isbyteZ x ->
                      HP.HMAC_SHA256.sixtyfour x = 
                      map Byte.unsigned (HP.HMAC_SHA256.sixtyfour (Byte.repr x)).
@@ -19,30 +20,30 @@ Proof. intros. unfold HP.HMAC_SHA256.sixtyfour.
  rewrite Byte.unsigned_repr; trivial. destruct H. 
  assert (BMU: Byte.max_unsigned = 255). reflexivity. omega.
 Qed.
-
+*)
 Lemma str_to_Z_length: forall k, 
       String.length k = length (str_to_Z k).
 Proof. intros. induction k; simpl; auto. Qed.
 
 Lemma first64_sixtyfour {A} (a:A): 
-      firstn 64 (HP.HMAC_SHA256.sixtyfour a) = HP.HMAC_SHA256.sixtyfour a.
+      firstn 64 (HMAC_SHA256.sixtyfour a) = HMAC_SHA256.sixtyfour a.
 Proof. apply firstn_precise. simpl. reflexivity. Qed. 
 
-Lemma length_SF {A} (x:A): length (HP.HMAC_SHA256.sixtyfour x) = 64%nat.
+Lemma length_SF {A} (x:A): length (HMAC_SHA256.sixtyfour x) = 64%nat.
 Proof.
-  unfold HP.HMAC_SHA256.sixtyfour.
+  unfold HMAC_SHA256.sixtyfour.
   rewrite length_list_repeat; trivial.
 Qed.
 
-Lemma Zlength_mkArgZ k pad: Zlength (HP.HMAC_SHA256.mkArgZ k pad) = Z.of_nat (min (length k) 64).
+Lemma Zlength_mkArgZ k pad: Zlength (HMAC_SHA256.mkArgZ k pad) = Z.of_nat (min (length k) 64).
 Proof. intros. repeat rewrite Zlength_correct.
-   unfold HP.HMAC_SHA256.mkArgZ, HP.HMAC_SHA256.mkArg, HP.HMAC_SHA256.sixtyfour.
+   unfold HMAC_SHA256.mkArgZ, HMAC_SHA256.mkArg, HMAC_SHA256.sixtyfour.
    repeat rewrite map_length. 
    rewrite combine_length, length_list_repeat . trivial.
 Qed.
 
-Lemma zeropad_isbyteZ: forall l, Forall isbyteZ l -> Forall isbyteZ (HP.HMAC_SHA256.zeroPad l).
-Proof. unfold isbyteZ, HP.HMAC_SHA256.zeroPad; intros.
+Lemma zeropad_isbyteZ: forall l, Forall isbyteZ l -> Forall isbyteZ (HMAC_SHA256.zeroPad l).
+Proof. unfold isbyteZ, HMAC_SHA256.zeroPad; intros.
   rewrite Forall_forall in *. intros.
   apply in_app_or in H0.
   destruct H0. apply (H _ H0).
@@ -50,8 +51,8 @@ Proof. unfold isbyteZ, HP.HMAC_SHA256.zeroPad; intros.
 Qed.
 
 Lemma nth_zeropad_left {d d'}: forall l i (I: 0<= i < Zlength l),
-      nth (Z.to_nat i) (HP.HMAC_SHA256.zeroPad l) d = nth (Z.to_nat i) l d'.
-Proof. unfold HP.HMAC_SHA256.zeroPad. intros.
+      nth (Z.to_nat i) (HMAC_SHA256.zeroPad l) d = nth (Z.to_nat i) l d'.
+Proof. unfold HMAC_SHA256.zeroPad. intros.
   destruct I.
   apply Z2Nat.inj_lt in H0; try omega.
   rewrite Zlength_correct, Nat2Z.id in H0.
@@ -61,15 +62,15 @@ Qed.
 
 Lemma mkKey_left {d d'}: forall l (L: false = (Zlength l >? 64)) 
         i (I: 0<= i < Zlength l),
-      nth (Z.to_nat i) (HP.HMAC_SHA256.mkKey l) d = nth (Z.to_nat i) l d'.
+      nth (Z.to_nat i) (HMAC_SHA256.mkKey l) d = nth (Z.to_nat i) l d'.
 Proof.
-  unfold HP.HMAC_SHA256.mkKey. intros. simpl. rewrite <- L.
+  unfold HMAC_SHA256.mkKey. intros. simpl. rewrite <- L.
   apply nth_zeropad_left; trivial.
 Qed.
 
 Lemma nth_zeropad_right {d} l i (I: Zlength l <= i < 64):
-      nth (Z.to_nat i) (HP.HMAC_SHA256.zeroPad l) d = Z0.
-Proof. unfold HP.HMAC_SHA256.zeroPad. 
+      nth (Z.to_nat i) (HMAC_SHA256.zeroPad l) d = Z0.
+Proof. unfold HMAC_SHA256.zeroPad. 
   specialize (Zlength_nonneg l). intros.
   rewrite app_nth2. rewrite nth_list_repeat'. trivial.
   apply minus_lt_compat_r. destruct I. apply Z2Nat.inj_lt in H1. apply H1.
@@ -85,55 +86,55 @@ Qed.
 
 Lemma mkKey_right {d}: forall l (L: false = (Zlength l >? 64)) 
         i (I: Zlength l <= i < 64),
-      nth (Z.to_nat i) (HP.HMAC_SHA256.mkKey l) d = Z0.
+      nth (Z.to_nat i) (HMAC_SHA256.mkKey l) d = Z0.
 Proof.
-  unfold HP.HMAC_SHA256.mkKey. intros. simpl. rewrite <- L.
+  unfold HMAC_SHA256.mkKey. intros. simpl. rewrite <- L.
   apply nth_zeropad_right; trivial.
 Qed.
 
-Lemma zeroPad_BlockSize: forall k, (length k <= HP.SHA256.BlockSize)%nat ->
-  length (HP.HMAC_SHA256.zeroPad k) = HP.SHA256.BlockSize%nat.
-Proof. unfold HP.HMAC_SHA256.zeroPad. intros. rewrite app_length, (*length_Nlist*) length_list_repeat. omega. 
+Lemma zeroPad_BlockSize: forall k, (length k <= SHA256.BlockSize)%nat ->
+  length (HMAC_SHA256.zeroPad k) = SHA256.BlockSize%nat.
+Proof. unfold HMAC_SHA256.zeroPad. intros. rewrite app_length, (*length_Nlist*) length_list_repeat. omega. 
 Qed. 
 
 Lemma length_SHA256': forall l, 
-  length (functional_prog.SHA_256' l) = HP.SHA256.DigestLength.
+  length (functional_prog.SHA_256' l) = SHA256.DigestLength.
 Proof. intros. unfold functional_prog.SHA_256'. simpl.
   rewrite length_intlist_to_Zlist, functional_prog.length_process_msg. reflexivity.
 Qed.
 
-Lemma mkKey_length l: length (HP.HMAC_SHA256.mkKey l) = HP.SHA256.BlockSize.
-Proof. intros. unfold HP.HMAC_SHA256.mkKey.
-  remember (Zlength l >? Z.of_nat HP.SHA256.BlockSize) as z. 
+Lemma mkKey_length l: length (HMAC_SHA256.mkKey l) = SHA256.BlockSize.
+Proof. intros. unfold HMAC_SHA256.mkKey.
+  remember (Zlength l >? Z.of_nat SHA256.BlockSize) as z. 
   destruct z. apply zeroPad_BlockSize.
     rewrite length_SHA256'.  
     apply Nat2Z.inj_le. simpl. omega. 
   apply zeroPad_BlockSize.
     rewrite Zlength_correct in Heqz. 
     apply Nat2Z.inj_le. 
-    specialize (Zgt_cases (Z.of_nat (Datatypes.length l)) (Z.of_nat HP.SHA256.BlockSize)). rewrite <- Heqz. trivial.
+    specialize (Zgt_cases (Z.of_nat (Datatypes.length l)) (Z.of_nat SHA256.BlockSize)). rewrite <- Heqz. trivial.
 Qed.
 
-Lemma mkKey_atBlockSize s: length s = HP.SHA256.BlockSize%nat ->
-      HP.HMAC_SHA256.mkKey s = s.
-Proof. unfold HP.HMAC_SHA256.mkKey. rewrite Zlength_correct.
+Lemma mkKey_atBlockSize s: length s = SHA256.BlockSize%nat ->
+      HMAC_SHA256.mkKey s = s.
+Proof. unfold HMAC_SHA256.mkKey. rewrite Zlength_correct.
   intros. rewrite H.
-  simpl. unfold HP.HMAC_SHA256.zeroPad. rewrite H. simpl.
+  simpl. unfold HMAC_SHA256.zeroPad. rewrite H. simpl.
   apply app_nil_r.  
 Qed.
 
-Lemma isbyteZ_mkKey: forall l, Forall isbyteZ l -> Forall isbyteZ (HP.HMAC_SHA256.mkKey l).
+Lemma isbyteZ_mkKey: forall l, Forall isbyteZ l -> Forall isbyteZ (HMAC_SHA256.mkKey l).
 Proof. intros.
-  unfold HP.HMAC_SHA256.mkKey.
-  remember (Zlength l >? Z.of_nat HP.SHA256.BlockSize).
+  unfold HMAC_SHA256.mkKey.
+  remember (Zlength l >? Z.of_nat SHA256.BlockSize).
   destruct b.
-    apply zeropad_isbyteZ. apply HP.SHA256.Hash_isbyteZ. 
+    apply zeropad_isbyteZ. apply SHA256.Hash_isbyteZ. 
     apply zeropad_isbyteZ; trivial.
 Qed.
 
 Lemma isbyte_hmac ipad opad m k: 
-   Forall isbyteZ (HMAC_functional_prog.HP.HMAC_SHA256.HMAC ipad opad m k).
-Proof. apply HP.SHA256.Hash_isbyteZ.  Qed.
+   Forall isbyteZ (HMAC_SHA256.HMAC ipad opad m k).
+Proof. apply SHA256.Hash_isbyteZ.  Qed.
 
 Lemma updAbs_len: forall L s t, update_abs L s t -> s256a_len t = s256a_len s + Zlength L * 8.
 Proof. intros. inversion H; clear H.
@@ -152,12 +153,12 @@ Proof. intros. inversion H; clear H.
   rewrite H; trivial.
 Qed.
 
-Lemma HMAC_length d k: length (HP.HMAC256 d k) = 32%nat.
+Lemma HMAC_length d k: length (HMAC256 d k) = 32%nat.
 Proof.
-  unfold HP.HMAC_SHA256.HMAC, HP.HMAC_SHA256.OUTER.
+  unfold HMAC_SHA256.HMAC, HMAC_SHA256.OUTER.
   apply length_SHA256'.
 Qed.
-Lemma HMAC_Zlength d k: Zlength (HP.HMAC256 d k) = 32.
+Lemma HMAC_Zlength d k: Zlength (HMAC256 d k) = 32.
 Proof.
   rewrite Zlength_correct, HMAC_length. reflexivity.
 Qed.
