sha/verif_hmacNK_crypto.v
@@ -14,6 +14,7 @@ Require Import sha.spec_sha.
 Require Import sha_lemmas.
 
 Require Import sha.HMAC_functional_prog.
+Require Import sha.HMAC256_functional_prog.
 Require Import sha.hmac_common_lemmas.
 Require Import ShaInstantiation.
 Require Import HMAC256_equivalence.
@@ -23,7 +24,7 @@ Require Import sha.hmac_NK.
 Require Import sha.spec_hmacNK.
 
 Lemma key_vector l:
-  length (bytesToBits (HP.HMAC_SHA256.mkKey l)) = b.
+  length (bytesToBits (HMAC_SHA256.mkKey l)) = b.
 Proof. rewrite bytesToBits_len, hmac_common_lemmas.mkKey_length; reflexivity. Qed.
 
 Definition mkCont (l:list Z) : HMAC_spec_abstract.HMAC_Abstract.Message (fun x => x=bytesToBits l /\ NPeano.divide 8 (length x)).
@@ -177,10 +178,10 @@ forward_call WITNESS.
     destruct H1 as [oS [InnSHA [OntSHA XX]]]. inversion XX; clear XX.
     subst.
       unfold innerShaInit in InnSHA. inversion InnSHA; clear InnSHA.
-      simpl in *. subst. unfold HP.HMAC_SHA256.mkArgZ, HP.HMAC_SHA256.mkArg in H9.
+      simpl in *. subst. unfold HMAC_SHA256.mkArgZ, HMAC_SHA256.mkArg in H9.
       assert (Zlength (map Byte.unsigned
         (map (fun p : byte * byte => Byte.xor (fst p) (snd p))
-           (combine (map Byte.repr (HP.HMAC_SHA256.mkKey key)) (HP.HMAC_SHA256.sixtyfour HP.Ipad))))
+           (combine (map Byte.repr (HMAC_SHA256.mkKey key)) (HMAC_SHA256.sixtyfour Ipad))))
         = Zlength (intlist_to_Zlist blocks ++ newfrag)).
         rewrite H9; reflexivity.
      clear H9.
@@ -188,7 +189,7 @@ forward_call WITNESS.
      rewrite Zlength_correct in *. rewrite map_length, combine_length in H1.
      rewrite app_length in H1.
      rewrite map_length, mkKey_length in H1.
-     unfold HP.SHA256.BlockSize, HP.HMAC_SHA256.sixtyfour in H1.
+     unfold SHA256.BlockSize, HMAC_SHA256.sixtyfour in H1.
      rewrite length_list_repeat, length_intlist_to_Zlist in H1. unfold WORD.
      rewrite Nat2Z.inj_add, Nat2Z.inj_mul, Z.mul_comm in H1. simpl in H1.
      unfold bitlength. repeat rewrite Zlength_correct. unfold WORD. rewrite <- H1. simpl. trivial.
