sha/verif_hmac_init_part2.v
@@ -7,6 +7,7 @@ Local Open Scope logic.
 Require Import sha.spec_sha.
 Require Import sha.sha_lemmas.
 Require Import sha.HMAC_functional_prog.
+Require Import sha.HMAC256_functional_prog.
 Require Import sha.spec_hmac.
 Require Import vst_lemmas.
 Require Import hmac_pure_lemmas.
@@ -89,46 +90,46 @@ Qed.
 Lemma UPD_IPAD: forall
   (key : list Z)
   (ZLI : Zlength
-        (HP.HMAC_SHA256.mkArgZ (map Byte.repr (HP.HMAC_SHA256.mkKey key)) HP.Ipad) =
+        ( HMAC_SHA256.mkArgZ (map Byte.repr (HMAC_SHA256.mkKey key)) Ipad) =
       64)
   (i : Z)
   (I : 0 <= i < 64)
-  (isbyteZQb : isbyteZ (nth (Z.to_nat i) (HP.HMAC_SHA256.mkKey key) 0))
-  (X : Znth i (map Vint (map Int.repr (HP.HMAC_SHA256.mkKey key))) Vundef =
-      Vint (Int.repr (nth (Z.to_nat i) (HP.HMAC_SHA256.mkKey key) 0))),
+  (isbyteZQb : isbyteZ (nth (Z.to_nat i) (HMAC_SHA256.mkKey key) 0))
+  (X : Znth i (map Vint (map Int.repr (HMAC_SHA256.mkKey key))) Vundef =
+      Vint (Int.repr (nth (Z.to_nat i) (HMAC_SHA256.mkKey key) 0))),
 upd_reptype_array tuchar i
   (FIRSTN i
      (map Vint
         (map Int.repr
            (map Byte.unsigned
-              (HP.HMAC_SHA256.mkArg (map Byte.repr (HP.HMAC_SHA256.mkKey key)) HP.Ipad)))))
+              (HMAC_SHA256.mkArg (map Byte.repr (HMAC_SHA256.mkKey key)) Ipad)))))
   (force_val
      (sem_cast_i2i I8 Unsigned
         (Vint
-           (Int.repr (Z.lxor (nth (Z.to_nat i) (HP.HMAC_SHA256.mkKey key) 0) 54))))) =
+           (Int.repr (Z.lxor (nth (Z.to_nat i) (HMAC_SHA256.mkKey key) 0) 54))))) =
 FIRSTN (i + 1)
   (map Vint
      (map Int.repr
         (map Byte.unsigned
-           (HP.HMAC_SHA256.mkArg (map Byte.repr (HP.HMAC_SHA256.mkKey key)) HP.Ipad)))).
+           (HMAC_SHA256.mkArg (map Byte.repr (HMAC_SHA256.mkKey key)) Ipad)))).
 Proof. intros.
-           assert (ZLI': length (HP.HMAC_SHA256.mkArgZ (map Byte.repr (HP.HMAC_SHA256.mkKey key)) HP.Ipad) = Z.to_nat 64).
+           assert (ZLI': length (HMAC_SHA256.mkArgZ (map Byte.repr (HMAC_SHA256.mkKey key)) Ipad) = Z.to_nat 64).
               rewrite Zlength_correct in ZLI. rewrite <- ZLI. rewrite Nat2Z.id; trivial.
            unfold FIRSTN. unfold upd_reptype_array.
-           rewrite skipn_short. Focus 2. rewrite firstn_length. unfold  HP.HMAC_SHA256.mkArgZ in ZLI'.
+           rewrite skipn_short. Focus 2. rewrite firstn_length. unfold  HMAC_SHA256.mkArgZ in ZLI'.
                                          do 2 rewrite map_length. rewrite ZLI'.
                                          rewrite Min.min_l. unfold nat_of_Z. rewrite Z2Nat.inj_add. simpl. omega. apply I. omega.
                                 apply Z2Nat.inj_le; omega.
-           rewrite force_lengthn_id. Focus 2. rewrite firstn_length. unfold  HP.HMAC_SHA256.mkArgZ in ZLI'.
+           rewrite force_lengthn_id. Focus 2. rewrite firstn_length. unfold  HMAC_SHA256.mkArgZ in ZLI'.
                                          do 2 rewrite map_length. rewrite ZLI'.
                                          rewrite Min.min_l. reflexivity.
                                 apply Z2Nat.inj_le; omega.
            rewrite Z2Nat.inj_add; try omega. rewrite <- firstn_app. f_equal.
           rewrite <- firstn_1_skipn with (d:=Vint (Int.repr (Byte.unsigned ((fun p : byte * byte => Byte.xor (fst p) (snd p)) (Byte.zero,Byte.zero))))).
-          Focus 2. do 2 rewrite map_length. unfold  HP.HMAC_SHA256.mkArgZ in ZLI'. rewrite ZLI'. apply Z2Nat.inj_lt; omega.
-          f_equal. rewrite map_nth. rewrite map_nth. rewrite map_nth. unfold Znth in X. unfold HP.HMAC_SHA256.mkArg.
+          Focus 2. do 2 rewrite map_length. unfold  HMAC_SHA256.mkArgZ in ZLI'. rewrite ZLI'. apply Z2Nat.inj_lt; omega.
+          f_equal. rewrite map_nth. rewrite map_nth. rewrite map_nth. unfold Znth in X. unfold HMAC_SHA256.mkArg.
                    rewrite (map_nth (fun p : byte * byte => Byte.xor (fst p) (snd p))
-                                       (combine (map Byte.repr (HP.HMAC_SHA256.mkKey key)) (HP.HMAC_SHA256.sixtyfour HP.Ipad)) 
+                                       (combine (map Byte.repr (HMAC_SHA256.mkKey key)) (HMAC_SHA256.sixtyfour Ipad)) 
                                        (Byte.zero, Byte.zero)
                                        (Z.to_nat i)).
                    rewrite combine_nth. 
@@ -136,16 +137,16 @@ Proof. intros.
                    assert (BMU: Byte.max_unsigned = 255). reflexivity.
                    assert (isByte54: 0 <= 54 <= Byte.max_unsigned).
                       rewrite BMU; omega. 
-                   destruct (isbyteZ_xor (nth (Z.to_nat i) (HP.HMAC_SHA256.mkKey key) 0) 54 isbyteZQb) as [AA BB].
+                   destruct (isbyteZ_xor (nth (Z.to_nat i) (HMAC_SHA256.mkKey key) 0) 54 isbyteZQb) as [AA BB].
                      split; rewrite BMU in *; omega.                      
                    unfold force_val. rewrite sem_cast_i2i_correct_range.
-                   destruct (zlt i 0); try omega. remember (HP.HMAC_SHA256.sixtyfour HP.Ipad).  simpl.
-                   rewrite (map_nth Byte.repr (HP.HMAC_SHA256.mkKey key) Z0).
+                   destruct (zlt i 0); try omega. remember (HMAC_SHA256.sixtyfour Ipad).  simpl.
+                   rewrite (map_nth Byte.repr (HMAC_SHA256.mkKey key) Z0).
                    unfold Byte.xor.
                    assert (NTH: nth (Z.to_nat i) l Byte.zero = Byte.repr 54).
                      subst l. apply nth_list_repeat'. apply (Z2Nat.inj_lt _ 64). apply I. omega. omega.
                    rewrite NTH, (Byte.unsigned_repr 54); trivial.
-                   rewrite (Byte.unsigned_repr (nth (Z.to_nat i) (HP.HMAC_SHA256.mkKey key) 0)).
+                   rewrite (Byte.unsigned_repr (nth (Z.to_nat i) (HMAC_SHA256.mkKey key) 0)).
                      Focus 2. destruct isbyteZQb. omega.
                    rewrite Byte.unsigned_repr. trivial.
                    rewrite BMU in *; split; omega. 
@@ -155,64 +156,64 @@ Qed.
 
 Lemma UPD_OPAD: forall
   (key : list Z)
-  (ZLI : Zlength (HP.HMAC_SHA256.mkArgZ (map Byte.repr (HP.HMAC_SHA256.mkKey key)) HP.Ipad) = 64)
-  (ZLO : Zlength (HP.HMAC_SHA256.mkArgZ (map Byte.repr (HP.HMAC_SHA256.mkKey key)) HP.Opad) = 64)
+  (ZLI : Zlength (HMAC_SHA256.mkArgZ (map Byte.repr (HMAC_SHA256.mkKey key)) Ipad) = 64)
+  (ZLO : Zlength (HMAC_SHA256.mkArgZ (map Byte.repr (HMAC_SHA256.mkKey key)) Opad) = 64)
   (i : Z)
   (I : 0 <= i < 64)
-  (isbyteZQb : isbyteZ (nth (Z.to_nat i) (HP.HMAC_SHA256.mkKey key) 0))
-  (X : Znth i (map Vint (map Int.repr (HP.HMAC_SHA256.mkKey key))) Vundef =
-       Vint (Int.repr (nth (Z.to_nat i) (HP.HMAC_SHA256.mkKey key) 0))),
+  (isbyteZQb : isbyteZ (nth (Z.to_nat i) (HMAC_SHA256.mkKey key) 0))
+  (X : Znth i (map Vint (map Int.repr (HMAC_SHA256.mkKey key))) Vundef =
+       Vint (Int.repr (nth (Z.to_nat i) (HMAC_SHA256.mkKey key) 0))),
 upd_reptype_array tuchar i
   (FIRSTN i
      (map Vint
         (map Int.repr
            (map Byte.unsigned
-              (HP.HMAC_SHA256.mkArg (map Byte.repr (HP.HMAC_SHA256.mkKey key)) HP.Opad)))) ++
+              (HMAC_SHA256.mkArg (map Byte.repr (HMAC_SHA256.mkKey key)) Opad)))) ++
    SKIPN i
      (map Vint
         (map Int.repr
            (map Byte.unsigned
-              (HP.HMAC_SHA256.mkArg (map Byte.repr (HP.HMAC_SHA256.mkKey key)) HP.Ipad)))))
+              (HMAC_SHA256.mkArg (map Byte.repr (HMAC_SHA256.mkKey key)) Ipad)))))
   (Vint
      (Int.zero_ext 8
         (Int.xor (Int.repr 92)
-           (Int.repr (nth (Z.to_nat i) (HP.HMAC_SHA256.mkKey key) 0))))) =
+           (Int.repr (nth (Z.to_nat i) (HMAC_SHA256.mkKey key) 0))))) =
 FIRSTN (i + 1)
   (map Vint
      (map Int.repr
         (map Byte.unsigned
-           (HP.HMAC_SHA256.mkArg (map Byte.repr (HP.HMAC_SHA256.mkKey key)) HP.Opad)))) ++
+           (HMAC_SHA256.mkArg (map Byte.repr (HMAC_SHA256.mkKey key)) Opad)))) ++
 SKIPN (i + 1)
   (map Vint
      (map Int.repr
         (map Byte.unsigned
-           (HP.HMAC_SHA256.mkArg (map Byte.repr (HP.HMAC_SHA256.mkKey key)) HP.Ipad)))).
+           (HMAC_SHA256.mkArg (map Byte.repr (HMAC_SHA256.mkKey key)) Ipad)))).
 Proof. intros.
-           assert (ZLI': length (HP.HMAC_SHA256.mkArgZ (map Byte.repr (HP.HMAC_SHA256.mkKey key)) HP.Ipad) = Z.to_nat 64).
+           assert (ZLI': length (HMAC_SHA256.mkArgZ (map Byte.repr (HMAC_SHA256.mkKey key)) Ipad) = Z.to_nat 64).
                  rewrite Zlength_correct in ZLI. rewrite <- ZLI. rewrite Nat2Z.id; trivial. 
-           assert (ZLO': length (HP.HMAC_SHA256.mkArgZ (map Byte.repr (HP.HMAC_SHA256.mkKey key)) HP.Opad) = Z.to_nat 64).
+           assert (ZLO': length (HMAC_SHA256.mkArgZ (map Byte.repr (HMAC_SHA256.mkKey key)) Opad) = Z.to_nat 64).
               rewrite Zlength_correct in ZLO. rewrite <- ZLO. rewrite Nat2Z.id; trivial.
            unfold FIRSTN. unfold upd_reptype_array, nat_of_Z.
            rewrite force_lengthn_long.
            Focus 2. unfold SKIPN; rewrite app_length, firstn_length, skipn_length.
-           unfold HP.HMAC_SHA256.mkArgZ in ZLI', ZLO'. 
+           unfold HMAC_SHA256.mkArgZ in ZLI', ZLO'. 
            do 2 rewrite map_length. rewrite ZLO'. 
            do 2 rewrite map_length. rewrite ZLI', Min.min_l. 2: apply Z2Nat.inj_le; omega.
               rewrite le_plus_minus_r; apply Z2Nat.inj_le; omega. 
-           do 2 rewrite map_length. unfold HP.HMAC_SHA256.mkArgZ in ZLI'; rewrite ZLI'. apply Z2Nat.inj_le; omega.
+           do 2 rewrite map_length. unfold HMAC_SHA256.mkArgZ in ZLI'; rewrite ZLI'. apply Z2Nat.inj_le; omega.
            rewrite firstn_app1.
            Focus 2. rewrite firstn_length, Min.min_l. omega.   
-              do 2 rewrite map_length. unfold HP.HMAC_SHA256.mkArgZ in ZLO'; rewrite ZLO'. apply Z2Nat.inj_le; omega.
+              do 2 rewrite map_length. unfold HMAC_SHA256.mkArgZ in ZLO'; rewrite ZLO'. apply Z2Nat.inj_le; omega.
            rewrite firstn_precise. 
            Focus 2. rewrite firstn_length, Min.min_l. omega.   
-              do 2 rewrite map_length. unfold HP.HMAC_SHA256.mkArgZ in ZLO'; rewrite ZLO'. apply Z2Nat.inj_le; omega.
+              do 2 rewrite map_length. unfold HMAC_SHA256.mkArgZ in ZLO'; rewrite ZLO'. apply Z2Nat.inj_le; omega.
            rewrite Z2Nat.inj_add; try omega. rewrite <- firstn_app. rewrite <- app_assoc.
            f_equal.
           rewrite <- firstn_1_skipn with (d:=Vint (Int.repr (Byte.unsigned ((fun p : byte * byte => Byte.xor (fst p) (snd p)) (Byte.zero,Byte.zero))))).
-          Focus 2. do 2 rewrite map_length. unfold  HP.HMAC_SHA256.mkArgZ in ZLO'. rewrite ZLO'. apply Z2Nat.inj_lt; omega.
-          simpl. f_equal. rewrite map_nth. rewrite map_nth. rewrite map_nth. unfold Znth in X. unfold HP.HMAC_SHA256.mkArg.
+          Focus 2. do 2 rewrite map_length. unfold  HMAC_SHA256.mkArgZ in ZLO'. rewrite ZLO'. apply Z2Nat.inj_lt; omega.
+          simpl. f_equal. rewrite map_nth. rewrite map_nth. rewrite map_nth. unfold Znth in X. unfold HMAC_SHA256.mkArg.
                    specialize (map_nth (fun p : byte * byte => Byte.xor (fst p) (snd p))
-                                       (combine (map Byte.repr (HP.HMAC_SHA256.mkKey key)) (HP.HMAC_SHA256.sixtyfour HP.Opad)) 
+                                       (combine (map Byte.repr (HMAC_SHA256.mkKey key)) (HMAC_SHA256.sixtyfour Opad)) 
                                        (Byte.zero, Byte.zero)
                                        (Z.to_nat i)). simpl; intros. rewrite H; clear H.
                    rewrite combine_nth. 
@@ -220,18 +221,18 @@ Proof. intros.
                    assert (BMU: Byte.max_unsigned = 255). reflexivity.
                    assert (isByte54: 0 <= 54 <= Byte.max_unsigned).
                       rewrite BMU; omega. 
-                   destruct (isbyteZ_xor (nth (Z.to_nat i) (HP.HMAC_SHA256.mkKey key) 0) 92 isbyteZQb) as [AA BB].
+                   destruct (isbyteZ_xor (nth (Z.to_nat i) (HMAC_SHA256.mkKey key) 0) 92 isbyteZQb) as [AA BB].
                      split; rewrite BMU in *; omega.
                    rewrite fst_unfold, snd_unfold, Int.xor_commut.
 (*                   unfold force_val. rewrite sem_cast_i2i_correct_range.
                    destruct (zlt i 0); try omega.*) 
-                   remember (HP.HMAC_SHA256.sixtyfour HP.Opad). 
-                   rewrite (map_nth Byte.repr (HP.HMAC_SHA256.mkKey key) Z0).
+                   remember (HMAC_SHA256.sixtyfour Opad). 
+                   rewrite (map_nth Byte.repr (HMAC_SHA256.mkKey key) Z0).
                    unfold Byte.xor.
                    assert (NTH: nth (Z.to_nat i) l Byte.zero = Byte.repr 92).
                      subst l. apply nth_list_repeat'. apply (Z2Nat.inj_lt _ 64). apply I. omega. omega.
                    rewrite NTH, (Byte.unsigned_repr 92); trivial.
-                   rewrite (Byte.unsigned_repr (nth (Z.to_nat i) (HP.HMAC_SHA256.mkKey key) 0)).
+                   rewrite (Byte.unsigned_repr (nth (Z.to_nat i) (HMAC_SHA256.mkKey key) 0)).
                      Focus 2. destruct isbyteZQb. omega.
                    rewrite Byte.unsigned_repr. unfold Int.xor.
                    rewrite Int.unsigned_repr.  
@@ -242,18 +243,18 @@ Proof. intros.
                    rewrite BMU in *; split; omega.
               rewrite <- skipn_skipn. 
               rewrite skipn_app2; rewrite firstn_length, Min.min_l.
-              Focus 2. do 2 rewrite map_length. unfold HP.HMAC_SHA256.mkArgZ in ZLO'; rewrite ZLO'.
+              Focus 2. do 2 rewrite map_length. unfold HMAC_SHA256.mkArgZ in ZLO'; rewrite ZLO'.
                        apply Z2Nat.inj_le; omega.
               rewrite minus_diag. simpl. unfold SKIPN. rewrite Z2Nat.inj_add, <- skipn_skipn. reflexivity.
               omega. omega. omega.
-              do 2 rewrite map_length. unfold HP.HMAC_SHA256.mkArgZ in ZLO'; rewrite ZLO'.
+              do 2 rewrite map_length. unfold HMAC_SHA256.mkArgZ in ZLO'; rewrite ZLO'.
                        apply Z2Nat.inj_le; omega.
 Qed.
 
 Definition postResetHMS key (iS oS: s256state): hmacstate :=
   (emptySha, (iS, (oS, 
    (if zlt 64 (Zlength key) then Vint (Int.repr 32) else Vint (Int.repr (Zlength key)), 
-   map Vint (map Int.repr (HP.HMAC_SHA256.mkKey key)))))).
+   map Vint (map Int.repr (HMAC_SHA256.mkKey key)))))).
 
 Definition initPostResetConditional r (c:val) (k: val) h key iS oS: mpred:=
   match k with
@@ -297,10 +298,10 @@ Lemma init_part2: forall
                       (EX  oSA : s256abs,
                        (EX  oS : s256state,
                         PROP 
-                        (innerShaInit (map Byte.repr (HP.HMAC_SHA256.mkKey key))
+                        (innerShaInit (map Byte.repr (HMAC_SHA256.mkKey key))
                            iSA /\
                          s256_relate iSA iS /\
-                         outerShaInit (map Byte.repr (HP.HMAC_SHA256.mkKey key))
+                         outerShaInit (map Byte.repr (HMAC_SHA256.mkKey key))
                            oSA /\ s256_relate oSA oS)
                         LOCAL  (`(eq pad) (eval_var _pad (tarray tuchar 64));
                         `(eq (Vptr cb cofs)) (eval_id _ctx);
@@ -447,22 +448,22 @@ Proof. intros.
 forward_if PostResetBranch. 
   { (* THEN*)
     (*remember (cVint (force_int oo ZnthV tuchar (map Vint (map Int.repr 
-              (map Byte.unsigned (HP.HMAC_SHA256.mkArg (map Byte.repr (HP.HMAC_SHA256.mkKey key)) HP.Ipad)))))) as IPADcont.
+              (map Byte.unsigned (HMAC_SHA256.mkArg (map Byte.repr (HMAC_SHA256.mkKey key)) Ipad)))))) as IPADcont.
     remember (cVint (force_int oo ZnthV tuchar (map Vint (map Int.repr 
-              (map Byte.unsigned (HP.HMAC_SHA256.mkArg (map Byte.repr (HP.HMAC_SHA256.mkKey key)) HP.Opad)))))) as OPADcont.
+              (map Byte.unsigned (HMAC_SHA256.mkArg (map Byte.repr (HMAC_SHA256.mkKey key)) Opad)))))) as OPADcont.
     *)
     remember (map Vint (map Int.repr 
-              (map Byte.unsigned (HP.HMAC_SHA256.mkArg (map Byte.repr (HP.HMAC_SHA256.mkKey key)) HP.Ipad)))) as IPADcont.
+              (map Byte.unsigned (HMAC_SHA256.mkArg (map Byte.repr (HMAC_SHA256.mkKey key)) Ipad)))) as IPADcont.
     remember (map Vint (map Int.repr 
-              (map Byte.unsigned (HP.HMAC_SHA256.mkArg (map Byte.repr (HP.HMAC_SHA256.mkKey key)) HP.Opad)))) as OPADcont.
-    assert (ZLI: Zlength (HP.HMAC_SHA256.mkArgZ (map Byte.repr (HP.HMAC_SHA256.mkKey key)) HP.Ipad) = 64).
+              (map Byte.unsigned (HMAC_SHA256.mkArg (map Byte.repr (HMAC_SHA256.mkKey key)) Opad)))) as OPADcont.
+    assert (ZLI: Zlength (HMAC_SHA256.mkArgZ (map Byte.repr (HMAC_SHA256.mkKey key)) Ipad) = 64).
             rewrite Zlength_mkArgZ.
             repeat rewrite map_length. rewrite mkKey_length.
-            unfold HP.SHA256.BlockSize; simpl. trivial. 
-    assert (ZLO: Zlength (HP.HMAC_SHA256.mkArgZ (map Byte.repr (HP.HMAC_SHA256.mkKey key)) HP.Opad) = 64).
+            unfold SHA256.BlockSize; simpl. trivial. 
+    assert (ZLO: Zlength (HMAC_SHA256.mkArgZ (map Byte.repr (HMAC_SHA256.mkKey key)) Opad) = 64).
             rewrite Zlength_mkArgZ.
             repeat rewrite map_length. rewrite mkKey_length.
-            unfold HP.SHA256.BlockSize; simpl. trivial. 
+            unfold SHA256.BlockSize; simpl. trivial. 
     (*remember (ZnthV tuchar (default_val (Tarray tuchar 64 noattr))) as DEFAULTcont.*)
     unfold data_at_, (*tuchars,*) tarray.
     (*erewrite data_at_array_at; try reflexivity. 2: omega.
@@ -550,18 +551,18 @@ forward_if PostResetBranch.
         (*eapply semax_pre0; [ apply now_later | ].
         eapply semax_post_flipped'.subst PostResetBranch.*)
         subst PostResetBranch.
-        assert (Xb: exists qb, nth (Z.to_nat i) (HP.HMAC_SHA256.mkKey key) Z0 = qb /\ isbyteZ qb).
-          { destruct (nth_mapIn (Z.to_nat i) (HP.HMAC_SHA256.mkKey key) 0) as [? [? ?]].
+        assert (Xb: exists qb, nth (Z.to_nat i) (HMAC_SHA256.mkKey key) Z0 = qb /\ isbyteZ qb).
+          { destruct (nth_mapIn (Z.to_nat i) (HMAC_SHA256.mkKey key) 0) as [? [? ?]].
              rewrite mkKey_length.
               split. apply (Z2Nat.inj_le 0); omega. apply (Z2Nat.inj_lt _ 64); omega.
             exists x; split; trivial. eapply Forall_forall. apply isbyteZ_mkKey. eassumption. eassumption.
           }
         destruct Xb as [qb [Qb isbyteZQb]].
-        assert (X: Znth i (map Vint (map Int.repr (HP.HMAC_SHA256.mkKey key))) Vundef
+        assert (X: Znth i (map Vint (map Int.repr (HMAC_SHA256.mkKey key))) Vundef
                    = Vint (Int.repr qb)). (* (Int.zero_ext 8 q)).*)
           { unfold Znth. destruct (zlt i 0). omega.
             rewrite nth_indep with (d':=Vint (Int.repr 0)).
-              Focus 2. repeat rewrite map_length. rewrite mkKey_length. unfold HP.SHA256.BlockSize; simpl. apply (Z2Nat.inj_lt _ 64); omega. 
+              Focus 2. repeat rewrite map_length. rewrite mkKey_length. unfold SHA256.BlockSize; simpl. apply (Z2Nat.inj_lt _ 64); omega. 
             repeat rewrite map_nth. rewrite Qb. trivial. 
           }
         (*unfold_data_at 2%nat. normalize. 
@@ -578,7 +579,7 @@ forward_if PostResetBranch.
         unfold force_val. rewrite sem_cast_i2i_correct_range.
             Focus 2. apply Znth_map_Vint_is_int_I8.
                      apply isbyteZ_mkKey. assumption.
-                     rewrite Zlength_correct, mkKey_length. unfold HP.SHA256.BlockSize; simpl; assumption.
+                     rewrite Zlength_correct, mkKey_length. unfold SHA256.BlockSize; simpl; assumption.
         rewrite X. 
         forward.
         normalize. subst x. unfold Int.xor. 
@@ -625,7 +626,7 @@ forward_if PostResetBranch.
     eapply semax_seq'.
     myframe_SEP'' [0; 5; 6].
     remember (init_s256abs, 
-            HP.HMAC_SHA256.mkArgZ (map Byte.repr (HP.HMAC_SHA256.mkKey key)) HP.Ipad,
+            HMAC_SHA256.mkArgZ (map Byte.repr (HMAC_SHA256.mkKey key)) Ipad,
             Vptr cb (Int.add cofs (Int.repr 108)),
             Vptr pb pofs, Tsh, 64, KV) as WITNESS.
     forward_call WITNESS.
@@ -640,15 +641,15 @@ forward_if PostResetBranch.
       cancel.
     }
     after_call. simpl. intros rho. subst WITNESS. rewrite firstn_precise. normalize.
-    unfold HP.HMAC_SHA256.mkArgZ, HP.HMAC_SHA256.mkArg. repeat rewrite map_length.
-      unfold HP.HMAC_SHA256.sixtyfour. 
+    unfold HMAC_SHA256.mkArgZ, HMAC_SHA256.mkArg. repeat rewrite map_length.
+      unfold HMAC_SHA256.sixtyfour. 
       rewrite combine_length, map_length, length_list_repeat, mkKey_length.
-      unfold HP.SHA256.BlockSize; simpl. trivial.
+      unfold SHA256.BlockSize; simpl. trivial.
 
     simpl.
     apply semax_pre with (P':=EX x : s256abs,
      (PROP  (update_abs
-          (HP.HMAC_SHA256.mkArgZ (map Byte.repr (HP.HMAC_SHA256.mkKey key)) HP.Ipad)
+          (HMAC_SHA256.mkArgZ (map Byte.repr (HMAC_SHA256.mkKey key)) Ipad)
           init_s256abs x)
      LOCAL  (
        `(eq (Vint (Int.repr 1))) (eval_id _reset);
@@ -659,14 +660,14 @@ forward_if PostResetBranch.
      SEP  (`(K_vector KV);
        `(sha256state_ x (Vptr cb (Int.add cofs (Int.repr 108))));
        `(data_block Tsh
-           (HP.HMAC_SHA256.mkArgZ (map Byte.repr (HP.HMAC_SHA256.mkKey key)) HP.Ipad)
+           (HMAC_SHA256.mkArgZ (map Byte.repr (HMAC_SHA256.mkKey key)) Ipad)
            (Vptr pb pofs));
       `(field_at Tsh t_struct_hmac_ctx_st [StructField _key_length]
          (if zlt 64 (Zlength key)
           then Vint (Int.repr 32)
           else Vint (Int.repr (Zlength key))) (Vptr cb cofs));
       `(field_at Tsh t_struct_hmac_ctx_st [StructField _key]
-          (map Vint (map Int.repr (HP.HMAC_SHA256.mkKey key))) (Vptr cb cofs));
+          (map Vint (map Int.repr (HMAC_SHA256.mkKey key))) (Vptr cb cofs));
       `(field_at Tsh t_struct_hmac_ctx_st [StructField _o_ctx] emptySha
           (Vptr cb cofs));
       `(field_at Tsh t_struct_hmac_ctx_st [StructField _md_ctx] emptySha
@@ -709,7 +710,7 @@ forward_if PostResetBranch.
         then Vint (Int.repr 32)
         else Vint (Int.repr (Zlength key))) (Vptr cb cofs));
    `(field_at Tsh t_struct_hmac_ctx_st [StructField _key]
-       (map Vint (map Int.repr (HP.HMAC_SHA256.mkKey key))) (Vptr cb cofs));
+       (map Vint (map Int.repr (HMAC_SHA256.mkKey key))) (Vptr cb cofs));
    
    `(data_at Tsh (Tarray tuchar 64 noattr) OPADcont (Vptr pb pofs));
 
@@ -740,7 +741,7 @@ forward_if PostResetBranch.
              then Vint (Int.repr 32)
              else Vint (Int.repr (Zlength key))) (Vptr cb cofs));
         `(field_at Tsh t_struct_hmac_ctx_st [StructField _key]
-           (map Vint (map Int.repr (HP.HMAC_SHA256.mkKey key))) (Vptr cb cofs));
+           (map Vint (map Int.repr (HMAC_SHA256.mkKey key))) (Vptr cb cofs));
          `(field_at Tsh t_struct_hmac_ctx_st [StructField _o_ctx] emptySha (Vptr cb cofs));
 (*        `(data_at Tsh (nested_field_type2 t_struct_hmac_ctx_st [StructField _o_ctx]) emptySha
            (Vptr cb
@@ -757,8 +758,8 @@ forward_if PostResetBranch.
         rewrite FIRSTN_precise.
          rewrite SKIPn_short. rewrite app_nil_r.
          cancel.
-         do 2 rewrite Zlength_map. unfold HP.HMAC_SHA256.mkArgZ in ZLI; rewrite ZLI. omega. 
-         do 2 rewrite Zlength_map. unfold HP.HMAC_SHA256.mkArgZ in ZLO; rewrite ZLO; trivial. 
+         do 2 rewrite Zlength_map. unfold HMAC_SHA256.mkArgZ in ZLI; rewrite ZLI. omega. 
+         do 2 rewrite Zlength_map. unfold HMAC_SHA256.mkArgZ in ZLO; rewrite ZLO; trivial. 
       }
       { (*unfold_data_at 3%nat. normalize. 
         rewrite (field_at_data_at Tsh t_struct_hmac_ctx_st [StructField _key]); try reflexivity.
@@ -771,18 +772,18 @@ forward_if PostResetBranch.
         2: simpl; rewrite Int.add_zero; reflexivity.*)
 (*        eapply semax_pre0; [ apply now_later | ].
         eapply semax_post_flipped'.*)
-        assert (Xb: exists qb, nth (Z.to_nat i) (HP.HMAC_SHA256.mkKey key) Z0 = qb /\ isbyteZ qb).
-          { destruct (nth_mapIn (Z.to_nat i) (HP.HMAC_SHA256.mkKey key) 0) as [? [? ?]].
+        assert (Xb: exists qb, nth (Z.to_nat i) (HMAC_SHA256.mkKey key) Z0 = qb /\ isbyteZ qb).
+          { destruct (nth_mapIn (Z.to_nat i) (HMAC_SHA256.mkKey key) 0) as [? [? ?]].
              rewrite mkKey_length.
               split. apply (Z2Nat.inj_le 0); omega. apply (Z2Nat.inj_lt _ 64); omega.
             exists x; split; trivial. eapply Forall_forall. apply isbyteZ_mkKey. eassumption. eassumption.
           }
         destruct Xb as [qb [Qb isbyteZQb]].
-        assert (X: Znth i (map Vint (map Int.repr (HP.HMAC_SHA256.mkKey key))) Vundef
+        assert (X: Znth i (map Vint (map Int.repr (HMAC_SHA256.mkKey key))) Vundef
                    = Vint (Int.repr qb)). (* (Int.zero_ext 8 q)).*)
           { unfold Znth. destruct (zlt i 0). omega.
             rewrite nth_indep with (d':=Vint (Int.repr 0)).
-              Focus 2. repeat rewrite map_length. rewrite mkKey_length. unfold HP.SHA256.BlockSize; simpl. apply (Z2Nat.inj_lt _ 64); omega. 
+              Focus 2. repeat rewrite map_length. rewrite mkKey_length. unfold SHA256.BlockSize; simpl. apply (Z2Nat.inj_lt _ 64); omega. 
             repeat rewrite map_nth. rewrite Qb. trivial. 
           }
         forward. entailer.
@@ -791,7 +792,7 @@ forward_if PostResetBranch.
         unfold force_val. rewrite sem_cast_i2i_correct_range.
         Focus 2. apply Znth_map_Vint_is_int_I8.
                      apply isbyteZ_mkKey. assumption.
-                     rewrite Zlength_correct, mkKey_length. unfold HP.SHA256.BlockSize; simpl; assumption.
+                     rewrite Zlength_correct, mkKey_length. unfold SHA256.BlockSize; simpl; assumption.
         rewrite X.
         forward.
         normalize. simpl. intros rho; entailer. cancel. (* 200MB memory consumption in this line!*)
@@ -817,7 +818,7 @@ forward_if PostResetBranch.
            then Vint (Int.repr 32)
            else Vint (Int.repr (Zlength key))) (Vptr cb cofs));
       `(data_at Tsh (nested_field_type2 t_struct_hmac_ctx_st [StructField _key])
-          (map Vint (map Int.repr (HP.HMAC_SHA256.mkKey key)))
+          (map Vint (map Int.repr (HMAC_SHA256.mkKey key)))
           (field_address t_struct_hmac_ctx_st [StructField _key] (Vptr cb cofs)));
       `(data_at Tsh (Tarray tuchar 64 noattr) OPADcont (Vptr pb pofs));
       `(data_at Tsh
@@ -859,7 +860,7 @@ forward_if PostResetBranch.
 (*    make_sequential.
     frame_SEP 0 1 3.*)
     remember (init_s256abs, 
-            HP.HMAC_SHA256.mkArgZ (map Byte.repr (HP.HMAC_SHA256.mkKey key)) HP.Opad,
+            HMAC_SHA256.mkArgZ (map Byte.repr (HMAC_SHA256.mkKey key)) Opad,
             Vptr cb (Int.add cofs (Int.repr 216)),
             Vptr pb pofs, Tsh, 64, KV) as WITNESS.
     forward_call WITNESS.
@@ -870,11 +871,11 @@ forward_if PostResetBranch.
                then Vint (Int.repr 32)
                else Vint (Int.repr (Zlength key))) (Vptr cb cofs));
          `(data_at Tsh (nested_field_type2 t_struct_hmac_ctx_st [StructField _key])
-              (map Vint (map Int.repr (HP.HMAC_SHA256.mkKey key)))
+              (map Vint (map Int.repr (HMAC_SHA256.mkKey key)))
                (Vptr cb (Int.add cofs
                   (Int.repr (nested_field_offset2 t_struct_hmac_ctx_st [StructField _key])))));
 (*         `(field_at Tsh t_struct_hmac_ctx_st [StructField _key]
-              (map Vint (map Int.repr (HP.HMAC_SHA256.mkKey key))) (Vptr cb cofs));*)
+              (map Vint (map Int.repr (HMAC_SHA256.mkKey key))) (Vptr cb cofs));*)
          `(field_at Tsh t_struct_hmac_ctx_st [StructField _md_ctx] emptySha (Vptr cb cofs));
          `(data_at Tsh (tarray tuchar (Zlength key)) (map Vint (map Int.repr key)) (Vptr kb kofs))]). 
         subst Frame. reflexivity.
